Symbolic evaluation for beta and normal order reduction is coming along well.  The proofs in bool are much nicer.  The churchnumScript.sml is broken until I get implement conditional rewriting in my rewriter for beta-reduction (should be easy).  The proofs there should become considerably nicer.

examples/lambda/barendregt/reductionEval.sig
@@ -3,5 +3,6 @@ sig
 
   val betafy : simpLib.simpset -> simpLib.simpset
   val unvarify_tac : Tactic.tactic
+  val NORMSTAR_ss : simpLib.ssfrag
 
 end
